upd

lawyer/nonblocking/examples/dequeue.v
@@ -4,7 +4,7 @@ From iris.bi.lib Require Import fixpoint.
 From trillium.program_logic Require Export weakestpre adequacy ectx_lifting.
 From fairness Require Import utils.
 From lawyer.examples Require Import obls_tactics.
-From lawyer.nonblocking.examples Require Import simple_queue_utils.
+From lawyer.nonblocking.examples Require Import simple_queue_utils simple_queue.
 From lawyer.obligations Require Import obligations_model obligations_resources obligations_am obligations_em obligations_logic env_helpers.
 From lawyer Require Import sub_action_em program_logic.
 From iris.algebra Require Import auth gmap gset excl excl_auth csum mono_nat.
@@ -13,465 +13,6 @@ From iris.base_logic.lib Require Import invariants.
 
 Close Scope Z.
 
-From iris.base_logic Require Export gen_heap.
-From iris.proofmode Require Import tactics coq_tactics.
-From iris.bi.lib Require Import fixpoint.
-From trillium.program_logic Require Export weakestpre adequacy ectx_lifting.
-From fairness Require Import utils.
-From lawyer.examples Require Import obls_tactics.
-From lawyer.nonblocking.examples Require Import simple_queue_utils.
-From lawyer.obligations Require Import obligations_model obligations_resources obligations_am obligations_em obligations_logic env_helpers.
-From lawyer Require Import sub_action_em program_logic.
-From iris.algebra Require Import auth gmap gset excl excl_auth csum mono_nat.
-From iris.base_logic.lib Require Import invariants.
-
-
-Class QueuePreG Σ := {
-  q_pre_max :: MaxExactPreG Σ;
-  q_pre_tok :: inG Σ (exclR unitO);
-  q_pre_hq :: HistQueuePreG Σ;
-  q_pre_rh :: ReadHistPreG Σ;
-  q_pre_rprot :: inG Σ (gmapUR nat read_state_cmra);
-  q_pre_dangle_rop :: inG Σ (excl_authUR (option nat));
-}.
-
-
-Record SimpleQueue := SQ {     
-    Head: loc; Tail: loc; BeingRead: loc; 
-    FreeLater: loc; OldHeadVal: loc;
-}.
-
-Class QueueG Σ := {
-    q_pre :: QueuePreG Σ; 
-    
-    q_hq :: HistQueueG Σ;
-    q_rh :: ReadHistG Σ;
-
-    q_sq: SimpleQueue;
-
-    q_γ_tok_rh: gname;
-    q_γ_tok_dq: gname;
-    q_γ_tok_cc: gname;
-    q_γ_tok_rop: gname;
-
-    q_γ_dangle: gname;
-    q_γ_rop: gname;
-
-    q_me_h :: MaxExactG Σ;
-    q_me_t :: MaxExactG Σ;
-    q_me_br :: MaxExactG Σ;
-    q_me_fl :: MaxExactG Σ;
-}.
-
-
-Definition get_val: val := λ: "nd", ! ("nd" +ₗ #0).
-Definition get_next: val := λ: "nd", ! ("nd" +ₗ #1).
-
-Definition free_el: val. Admitted.
-
-Definition get_to_free '(SQ _ _ BR FL _): val :=
-  λ: "ph",
-    if: ("ph" = !#BR)
-    then
-      let: "old_fl" := !#FL in
-      #FL <- "ph" ;;
-      "old_fl"
-    else "ph"
-.
-
-Definition dequeue '(SQ H T BR FL OHV as sq): val :=
-  λ: "q",
-    let: "c" := !#H in
-    if: ("c" = !#T)
-    then NONE
-    else
-      let: "v" := get_val "c" in
-      #OHV <- "v" ;;
-      #H <- (get_next "c") ;;
-      let: "to_free" := get_to_free sq "c" in
-      free_el "to_free" ;;
-      (SOME "v")
-.
-
-
-Section QueueResources. 
-
-  Context {Σ} {hG: heap1GS Σ} {iG: invGS_gen HasNoLc Σ}.
-  
-  Context {QL: QueueG Σ}.
-  
-  Definition hn_interp (hn: HistNode): iProp Σ :=
-    let '(l, (v, nxt)) := hn in
-    l ↦ v ∗ (l +ₗ 1) ↦ #nxt.
-
-  Definition dummy_node: Node := (#0, Loc 0).
-
-  Fixpoint is_LL_into (hq: HistQueue) (pt: loc) := 
-    match hq with 
-    | [] => True
-    | [ (_, (_, nxt)) ] => nxt = pt
-    (*   | (_, (_, nxt1)) :: ((l2, (_, _)) as hn2) :: hq' => nxt1 = l2 /\ is_LL (hn2 :: hq') *)
-    (** to avoid introducing Function *)
-    | (_, (_, nxt1)) :: hq' =>
-        match hq' with
-        | [] => True
-        | (l2, (_, _)) :: _ => nxt1 = l2 /\ is_LL_into hq' pt
-        end
-    end.
-
-  (** tail always points to a dummy node
-      which doesn NOT belong to the logical queue hq.
-      Upon enqueuing, this dummy note is updated and appended to hq.
-   *)
-  Definition phys_queue_interp (pq: HistQueue): iProp Σ :=
-    ([∗ list] nd ∈ pq, hn_interp nd) ∗
-    ∃ (pt: loc), Tail q_sq ↦ #pt ∗ hn_interp (pt, dummy_node) ∗ ⌜ is_LL_into pq pt ⌝ ∗
-    let ph: loc := (from_option (fun hn => hn.1) pt (pq !! 0)) in
-    Head q_sq ↦{1/2} #ph
-  . 
-      
-  
-  Definition queue_interp (hq: HistQueue) (h t br fl: nat): iProp Σ :=
-    let pq := drop h hq in
-    ⌜ t = length hq ⌝ ∗ 
-    (* ([∗ list] nd ∈ pq, hn_interp nd) ∗ *)
-    (* ∃ (pt: loc), Tail q_sq ↦ #pt ∗ hn_interp (pt, dummy_node) ∗ ⌜ is_LL_into pq pt ⌝ ∗ *)
-    (* let ph: loc := (from_option (fun hn => hn.1) pt (hq !! h)) in *)
-    (* Head q_sq ↦{1/2} #ph ∗ *)
-    phys_queue_interp pq ∗ 
-    (∃ (nbr: HistNode), ⌜ hq !! br = Some nbr ⌝ ∗ BeingRead q_sq ↦#(nbr.1)) ∗
-    (∃ (nfl: HistNode), ⌜ hq !! fl = Some nfl ⌝ ∗ FreeLater q_sq ↦#(nfl.1) ∗ hn_interp nfl)
-  .
-
-  Lemma queue_interp_cur_empty (hq: HistQueue) (h br fl: nat):
-    queue_interp hq h h br fl -∗ ⌜ forall d, hq !! (h + d)%nat = None ⌝.
-  Proof using.
-    iIntros "(%&_)". subst. iPureIntro.
-    intros. apply lookup_ge_None_2. lia.
-  Qed.
-  
-  (* TODO: try to get rid of if *)
-  Global Instance hni_tl hn: Timeless (hn_interp hn).
-  Proof using.
-    destruct hn as [? [??]]. apply _.
-  Defined. 
-  
-  (* TODO: try to get rid of if *)
-  Global Instance qi_tl: forall hq h t br fl, Timeless (queue_interp hq h t br fl).
-  Proof using. 
-    intros. rewrite /queue_interp.
-    apply _. 
-  Defined.
-  
-  Definition dangle_auth (od: option nat): iProp Σ := own q_γ_dangle (●E od).
-  Definition dangle_frag (od: option nat): iProp Σ := own q_γ_dangle (◯E od).
-  
-  Definition rop_auth (rop: option nat): iProp Σ := own q_γ_rop (●E rop).
-  Definition rop_frag (rop: option nat): iProp Σ := own q_γ_rop (◯E rop).
-  
-  Definition dangle_interp (od: option nat) (h: nat) (hq: HistQueue): iProp Σ :=
-    dangle_auth od ∗ (⌜ od = None ⌝ ∨ ⌜ od = Some (h - 1) ⌝ ∗ from_option hn_interp (⌜ False ⌝)%I (hq !! (h - 1)))
-  . 
-  
-  Definition auths (h t br fl: nat): iProp Σ :=
-    @me_auth _ q_me_h h ∗ @me_auth _ q_me_t t ∗ @me_auth _ q_me_br br ∗
-    @me_auth _ q_me_fl fl
-  .
-
-  Definition snapshot (h t br fl: nat): iProp Σ :=
-    @me_lb _ q_me_h h ∗ @me_lb _ q_me_t t ∗ @me_lb _ q_me_br br ∗
-    @me_lb _ q_me_fl fl
-  .
-
-  Lemma take_snapshot (h t br fl: nat): 
-    auths h t br fl -∗ snapshot h t br fl.
-  Proof using.
-    iIntros "(?&?&?&?)".
-    rewrite /snapshot. repeat iSplit; by iApply @me_auth_save.
-  Qed.
-
-  Lemma snapshot_lb (h t br fl: nat) (h' t' br' fl': nat):
-    snapshot h t br fl -∗ auths h' t' br' fl' -∗
-    ⌜ h <= h' /\ t <= t' /\ br <= br' /\ fl <= fl'⌝.
-  Proof using.
-    iIntros "#(X&?&?&?) (Y&?&?&?)".
-    repeat iSplit.
-    all: iApply (@me_auth_lb with "[-]"); eauto.
-  Qed.
-    
-  Definition cancel_witness (r: nat): iProp Σ :=
-    ∃ r', ⌜ r < r' ⌝ ∗ @me_lb _ q_me_h r'.
-
-  Definition rop_token: iProp Σ := own q_γ_tok_rop (Excl ()).
-
-  Definition safe_read (r: nat) (h br fl: nat) (od: option nat) rp: iProp Σ :=
-    ⌜ r = h ⌝ ∗ (⌜ rp = rs_init ⌝ ∨ ⌜ r = br ⌝ ∗ ⌜ rp = rs_proc (Some rsp_going) ⌝ ∗ rop_token) ∨
-    ⌜ r = h - 1 /\ r = br /\ is_Some od ⌝ ∗ ⌜ rp = rs_proc (Some rsp_protected) ⌝ ∨
-    ⌜ r = br /\ r = fl ⌝ ∗  ⌜ rp = rs_proc (Some rsp_protected) ⌝
-  .
-
-  Definition rop_interp (rop: option nat) (h br fl: nat) (od: option nat): iProp Σ :=
-    ∀ i, ⌜ rop = Some i  ⌝ -∗ ∃ r rp, ith_read i r 0 ∗ ith_rp i rp ∗
-        (safe_read r h br fl od rp ∨ ⌜ rp = rs_canceled ⌝ ∗ cancel_witness r).
-  
-  Definition read_head_resources (t br: nat): iProp Σ :=
-    @me_exact _ q_me_t t ∗ @me_exact _ q_me_br br ∗ rop_frag None ∗ rop_token.
-
-  Definition dequeue_resources (h fl: nat) (ph: loc) (od: option nat): iProp Σ :=
-    @me_exact _ q_me_h h ∗ @me_exact _ q_me_fl fl ∗
-    Head q_sq ↦{1/2} #ph ∗ dangle_frag od. 
-  
-  Definition read_head_token: iProp Σ := own q_γ_tok_rh (Excl ()).
-  Definition dequeue_token: iProp Σ := own q_γ_tok_dq (Excl ()).
-
-  Definition hq_state_wf h t br fl: Prop :=
-    (* fl <= br /\ *) (* see runs.org for a counterexample *)
-    br <= h /\ fl < h /\ h <= t.
-    (* THIS IS FALSE: br can fall behind arbitrarily *)
-    (* (br = h \/ br = fl \/ od = Some (h - 1) /\ br = h - 1).  *)
-
-  Definition br_lb (b: nat) := @me_lb _ q_me_br b.
-
-  Definition read_hist_wf (hist: read_hist) (rop: option nat) (h: nat) :=
-    exists n, dom hist = set_seq 0 (S n) /\ (rop = None \/ rop = Some n) /\ 
-           (forall i j opi opj, i < j -> hist !! i = Some opi -> hist !! j = Some opj ->
-                           opi.1.2 <= opj.1.1) /\
-           (forall i opi, hist !! i = Some opi -> opi.1.1 <= h /\ opi.1.2 <= h).
-
-  Definition old_rps (hist: read_hist) (rop: option nat): iProp Σ :=
-    (* [∗ set] i ∈ (dom hist) ∖ (from_option (fun n => {[ n ]}) ∅ rop), *)
-    [∗ map] i ↦ '((r, b), rp) ∈ (from_option (fun n => delete n hist) hist rop),
-      (* (dom hist) ∖ (from_option (fun n => {[ n ]}) ∅ rop), *)
-      ∃ rp, ith_rp i rp ∗ ⌜ rs_fin rp ⌝ ∗
-              (* (⌜ rp ≠ rs_canceled ⌝ -∗ br_lb b) *)
-              br_lb r
-  . 
-
-  (* TODO: upstream, find existing? *)
-  Global Instance Persistent_pure_helper P (R: iProp Σ) `{Decision P}:
-    (P -> Persistent R) -> Persistent (R ∗ ⌜ P ⌝).
-  Proof using.
-    intros PR. destruct (decide P).
-    - apply bi.sep_persistent; try by apply _. by apply PR.
-    - unshelve eapply bi.Persistent_proper. 1: exact (False)%I.
-      2: apply _. 
-      iSplit.
-      + by iIntros "(_&%)".
-      + by iIntros "?".
-  Qed.
-
-  Global Instance old_rps_pers: forall hist rop, Persistent (old_rps hist rop).
-  Proof using.
-    intros. rewrite /old_rps. apply big_sepM_persistent.
-    intros ? [[??] ?] ITH. simpl. 
-    apply bi.exist_persistent. intros rp.
-    rewrite bi.sep_assoc bi.sep_comm bi.sep_assoc. 
-    apply Persistent_pure_helper; [apply _| ]. 
-    intros. destruct H as [-> | [-> | ->]]; apply _.
-  Qed.
-
-  Definition ohv_interp: iProp Σ := ∃ ohv, OldHeadVal q_sq↦ ohv.
-
-  Definition read_hist_interp hist rop h br fl od: iProp Σ :=
-    rop_auth rop ∗
-    rop_interp rop h br fl od ∗ read_hist_auth hist ∗
-    ⌜ read_hist_wf hist rop h ⌝ ∗ old_rps hist rop
-  . 
-  
-  Definition queue_inv_inner (hq: HistQueue) (h t br fl: nat)
-    (rop od: option nat) (hist: read_hist): iProp Σ :=
-    hq_auth hq ∗ auths h t br fl ∗ ⌜ hq_state_wf h t br fl ⌝ ∗
-    queue_interp hq h t br fl ∗ dangle_interp od h hq ∗ ohv_interp ∗
-    read_hist_interp hist rop h br fl od ∗ 
-    (read_head_resources t br ∨ read_head_token) ∗ 
-    ((∃ ph, dequeue_resources h fl ph None) ∨ dequeue_token)
-  .
-  
-  Definition queue_ns := nroot .@ "queue".
-
-  Definition queue_at (q: val): iProp Σ :=
-    ⌜ q = (#(Head q_sq), (#(Tail q_sq), (#(BeingRead q_sq), (#(FreeLater q_sq), #(OldHeadVal q_sq)))))%V ⌝. 
-  
-  (* Definition queue_inv (q: loc): iProp Σ := *)
-  Definition queue_inv (q: val): iProp Σ :=
-    queue_at q ∗ inv queue_ns 
-      (∃ hq h t br fl rop od hist, queue_inv_inner hq h t br fl rop od hist)
-  .
-  
-  Lemma dequeue_token_excl:
-    dequeue_token -∗ dequeue_token -∗ False.
-  Proof using.
-    simpl. 
-    rewrite bi.wand_curry -own_op.
-    iIntros "X". by iDestruct (own_valid with "[$]") as %V.
-  Qed. 
-    
-  Lemma dequeue_resources_excl h1 fl1 ph1 od1 h2 fl2 ph2 od2:
-    dequeue_resources h1 fl1 ph1 od1 -∗ dequeue_resources h2 fl2 ph2 od2 -∗ False.
-  Proof using.
-    simpl. rewrite /dequeue_resources.
-    iIntros "(X&_) (Y&_)".
-    by iApply (me_exact_excl with "X [$]"). 
-  Qed.
-
-  Lemma dequeue_resources_auth_agree h' fl' ph od h t br fl:
-    dequeue_resources h' fl' ph od -∗ auths h t br fl -∗ ⌜ h' = h /\ fl' = fl ⌝.
-  Proof using.
-    simpl. iIntros "(H&FL&?&?) (H'&?&?&FL')".
-    iDestruct (me_auth_exact with "H' H") as %?. 
-    iDestruct (me_auth_exact with "FL' FL") as %?.
-    done. 
-  Qed. 
-    
-  Lemma dangle_auth_frag_agree od1 od2:
-    dangle_auth od1 -∗ dangle_frag od2 -∗ ⌜ od2 = od1 ⌝. 
-  Proof using.
-    simpl. rewrite /dangle_auth /dangle_frag.
-    rewrite bi.wand_curry -own_op.
-    iIntros "X". iDestruct (own_valid with "[$]") as %V.
-    iPureIntro. symmetry. by apply excl_auth_agree_L.
-  Qed.  
-    
-  Lemma dangle_update od1 od2 od':
-    dangle_auth od1 -∗ dangle_frag od2 ==∗ dangle_auth od' ∗ dangle_frag od'. 
-  Proof using.
-    simpl. rewrite /dangle_auth /dangle_frag.
-    rewrite bi.wand_curry -!own_op.
-    iApply own_update. apply excl_auth_update. 
-  Qed.  
-    
-  Lemma dequeue_resources_dangle_agree h fl ph od od' h' hq':
-    dequeue_resources h fl ph od -∗ dangle_interp od' h' hq' -∗ ⌜ od' = od ⌝.
-  Proof using.
-    simpl. iIntros "(?&?&?&FRAG) (AUTH&?)".
-    by iDestruct (dangle_auth_frag_agree with "[$] [$]") as %?. 
-  Qed.
-    
-  Lemma dequeue_res_head_agree h fl (ph ph': loc) od:
-    dequeue_resources h fl ph od -∗ Head q_sq ↦{1 / 2} #ph' -∗ ⌜ ph' = ph ⌝.
-  Proof using.
-    simpl. rewrite /dequeue_resources. iIntros "(_&_&H'&?) H".
-    iDestruct (pointsto_agree with "[$] [$]") as %?. set_solver.
-  Qed.
-    
-  Lemma cancel_rop h t br fl h'
-    (LT: h' < h):
-    auths h t br fl -∗ cancel_witness h'.
-  Proof using.
-    iIntros "(H&?&?&?)".
-    rewrite /cancel_witness.
-    iDestruct (me_auth_save with "H") as "LB".
-    iExists _. by iFrame.
-  Qed.
-    
-  Lemma old_rps_olds hist n:
-    old_rps hist (Some n) ⊣⊢ old_rps (delete n hist) None.
-  Proof using.
-    rewrite /old_rps. simpl. done. 
-  Qed.
-    
-  Lemma br_lb_bound b h t br fl:
-    br_lb b -∗ auths h t br fl -∗ ⌜ b <= br ⌝.
-  Proof using.
-    iIntros "LB (?&?&BR&?)".
-    iApply (me_auth_lb with "BR LB").
-  Qed.  
-
-  Lemma hn_interp_ptr_excl ptr nd1 nd2:
-    hn_interp (ptr, nd1) -∗ hn_interp (ptr, nd2) -∗ False.
-  Proof using.
-    simpl. destruct nd1, nd2. iIntros "[P1 ?] [P2 ?]".
-    iCombine "P1 P2" as "P". iDestruct (pointsto_valid with "P") as %V.
-    done.
-  Qed.
-
-  Lemma access_queue_ends hq h t br fl:
-    hq_auth hq -∗ queue_interp hq h t br fl -∗
-      ∃ (ph pt: loc), Head q_sq ↦{1/2} #ph ∗ (Tail q_sq) ↦ #pt ∗
-        (⌜ h >= t /\ ph = pt ⌝ ∨ ⌜ h < t /\ ph ≠ pt ⌝ ∗ ∃ (nd: Node), ith_node h (ph, nd)) ∗
-        (Head q_sq ↦{1/2} #ph -∗ (Tail q_sq) ↦ #pt -∗ hq_auth hq ∗ queue_interp hq h t br fl).
-  Proof using.
-    simpl. iIntros "[AUTH #FRAGS] QI".
-    rewrite /queue_interp. iDestruct "QI" as "(%T_LEN & PQI & BR & FL)".
-    rewrite /phys_queue_interp. iDestruct "PQI" as "(Q & (%pt & TAIL & DUMMY & %LL & HEAD))".
-    
-    iFrame "HEAD TAIL".
-    rewrite lookup_drop Nat.add_0_r. 
-    destruct (Nat.lt_ge_cases h t) as [LT | GE]; subst t.     
-    - pose proof LT as [[ph [??]] HTH]%lookup_lt_is_Some_2.
-      rewrite HTH. simpl.
-      iDestruct (big_sepL_lookup_acc with "FRAGS") as "[ITH _]"; [by eauto| ].
-      iFrame "ITH BR". 
-
-      iDestruct (big_sepL_lookup_acc with "Q") as "[HNI CLOS]".
-      { erewrite lookup_drop. by erewrite Nat.add_0_r. }
-      iAssert (⌜ ph ≠ pt ⌝)%I as %NEQ.
-      { iIntros (<-). rewrite {1}/hn_interp.
-        iDestruct "DUMMY" as "[X _]". iDestruct "HNI" as "[Y _]".
-        iDestruct (pointsto_valid_2 with "[$] [$]") as %V. set_solver. }
-      iSplit; [iRight; done| ].
-      iSpecialize ("CLOS" with "[$]"). 
-      iIntros "??". by iFrame "#∗". 
-    - iSplit. 
-      2: { iIntros "??". by iFrame "#∗". }
-      iLeft. iSplit; [done| ].
-      rewrite (lookup_ge_None_2 _ h) /=; done.      
-  Qed.
-
-  Lemma access_queue hq h t br fl i hn
-    (IN: h <= i < t):
-    hq_auth hq -∗ queue_interp hq h t br fl -∗ ith_node i hn -∗
-    hn_interp hn ∗ (hn_interp hn -∗ queue_interp hq h t br fl ∗ hq_auth hq).
-  Proof using.
-    simpl. rewrite /queue_interp. iIntros "AUTH (% & PQI & $) #ITH".
-    rewrite /phys_queue_interp. iDestruct "PQI" as "(Q & (%pt & TAIL & DUMMY & %LL & HEAD))".
-    iDestruct (hq_auth_lookup with "[$] [$]") as %ITH.
-    apply proj1, Nat.le_sum in IN as [? ->].
-    iDestruct (big_sepL_lookup_acc with "Q") as "[HNI CLOS]".
-    { erewrite lookup_drop; eauto. }
-    iFrame. iIntros. iFrame. repeat iSplit; try done. by iApply "CLOS".     
-  Qed. 
-
-  (* (* TODO: also holds if h is not in the hist queue (e.g. initially) *) *)
-  (* Lemma queue_interp_ph_neq_pfl' (hq: HistQueue) h t br fl (ptr: loc): *)
-  (*   queue_interp hq h t br fl -∗ ⌜ exists nd, hq !! h = Some (ptr, nd) ⌝ -∗ *)
-  (*   ⌜ exists nd, hq !! fl = Some (ptr, nd) ⌝ -∗ *)
-  (*     False. *)
-  (* Proof using. *)
-  (*   simpl.  *)
-  (*   iIntros "QI (%ndh & %HTH) (%ndfl & %FLTH)". rewrite /queue_interp. *)
-  (*   rewrite /queue_interp. iDestruct "QI" as "(%T_LEN &  HNIS & %pt & TAIL & TLI & %LL & HEAD & BR & FL)". *)
-  (*   iDestruct "FL" as "(% & %FLTH_ & FL & HNI_FL)". *)
-  (*   rewrite FLTH in FLTH_. inversion FLTH_. subst. simpl. *)
-  (*   rewrite HTH. simpl. *)
-  (*   iDestruct (big_sepL_elem_of with "HNIS") as "II". *)
-  (*   { apply elem_of_list_lookup. eexists. *)
-  (*     erewrite lookup_drop with (i := 0). *)
-  (*     by rewrite Nat.add_0_r. } *)
-  (*   simpl. by iDestruct (hn_interp_ptr_excl with "[$] [$]") as "?". *)
-  (* Qed.     *)
-
-  Lemma queue_interp_dangle_neq_pfl' (hq: HistQueue) h t br fl (ptr: loc):
-    queue_interp hq h t br fl -∗
-     dangle_interp (Some (h - 1)) h hq -∗
-    ⌜ exists nd, hq !! fl = Some (ptr, nd) ⌝ -∗
-    ⌜ exists nd, hq !! (h - 1) = Some (ptr, nd) ⌝ -∗
-      False.
-  Proof using.
-    simpl. 
-    iIntros "QI DI (%ndfl & %FLTH) (% & %DTH)".
-    rewrite /queue_interp. iDestruct "QI" as "(%T_LEN & PQI & BR & FL)".
-    rewrite /phys_queue_interp. iDestruct "PQI" as "(Q & (%pt & TAIL & DUMMY & %LL & HEAD))".
-    iDestruct "FL" as "(% & %FLTH_ & FL & HNI_FL)".
-    rewrite FLTH in FLTH_. inversion FLTH_. subst. simpl.
-    rewrite /dangle_interp.
-    iDestruct "DI" as "(AUTH & [% | (_ & HNI)])".
-    { done. }
-    rewrite  DTH. simpl.
-    by iDestruct (hn_interp_ptr_excl with "[$] [$]") as "?".
-  Qed.
-
-End QueueResources.
 
 Section Dequeue.
 
@@ -1053,8 +594,7 @@ Section Dequeue.
     
     split_cps "CPS" get_loc_fuel.
     wp_bind (! _)%E. 
-    (* replace BeingRead with (simple_queue.BeingRead q_sq) by (by rewrite Q_SQ).  *)
-    replace BeingRead0 with (BeingRead q_sq) by (by rewrite Q_SQ).
+    replace BeingRead with (simple_queue.BeingRead q_sq) by (by rewrite Q_SQ).
     iApply (check_BR_spec with "[-POST CPS]").
     { apply READ_BOUND. }
     { iFrame "#∗". }
@@ -1078,8 +618,7 @@ Section Dequeue.
 
     wp_bind (! _)%E.
     split_cps "CPS" 1. rewrite -cp_mul_1.
-    (* replace FreeLater with (simple_queue.FreeLater q_sq) by (by rewrite Q_SQ).  *)
-    replace FreeLater0 with (FreeLater q_sq) by (by rewrite Q_SQ).
+    replace FreeLater with (simple_queue.FreeLater q_sq) by (by rewrite Q_SQ).
     iApply (read_FL_spec with "[-POST CPS]").
     { iFrame "#∗". }
     iIntros "!> %pfl (%ndfl & #FLTH & DR & PH)".
@@ -1251,8 +790,7 @@ Section Dequeue.
     
     iApply sswp_MU_wp; [done| ].
     iDestruct (access_queue_ends with "[$] [$]") as "(%ph & %pt & HEAD & TAIL & HT & CLOS')".
-    (* replace Head with (simple_queue.Head q_sq) by (by rewrite Q_SQ). *)
-    replace Head0 with (Head q_sq) by (by rewrite Q_SQ).
+    replace Head with (simple_queue.Head q_sq) by (by rewrite Q_SQ).
     iApply (wp_load with "HEAD"). iIntros "!> HEAD".
     iDestruct "DQ" as "[[%ph_ DR] | TOK']".
     2: { by iDestruct (dequeue_token_excl with "[$] [$]") as "?". }
@@ -1277,8 +815,7 @@ Section Dequeue.
     iDestruct "inv" as ">(HQ & AUTHS & %ORDER & QI & DANGLE & OHV & RHI & RH & DQ)".
     iApply sswp_MU_wp; [done| ].
     iDestruct (access_queue_ends with "[$] [$]") as "(%ph_ & %pt & HEAD & TAIL & #HT & CLOS')".
-    (* replace Tail with (simple_queue.Tail q_sq) by (by rewrite Q_SQ). *)
-    replace Tail0 with (Tail q_sq) by (by rewrite Q_SQ).
+    replace Tail with (simple_queue.Tail q_sq) by (by rewrite Q_SQ).
     iApply (wp_load with "[$]"). iIntros "!> TAIL".
     iDestruct (dequeue_res_head_agree with "DR [$]") as %->. 
     iDestruct (dequeue_resources_auth_agree with "DR [$]") as %[<- <-].
@@ -1333,8 +870,7 @@ Section Dequeue.
 
     destruct ndh as [vh nxh]. simpl.
     wp_bind (_ <- _)%E.
-    (* replace OldHeadVal with (simple_queue.OldHeadVal q_sq) by (by rewrite Q_SQ). *)
-    replace OldHeadVal0 with (OldHeadVal q_sq) by (by rewrite Q_SQ).
+    replace OldHeadVal with (simple_queue.OldHeadVal q_sq) by (by rewrite Q_SQ).
     split_cps "CPS" get_loc_fuel; [cbv; lia| ].     
     iApply (update_ohv_spec with "[$QAT $PH $CPS' $INV]").
     iIntros "!> PH".
@@ -1351,7 +887,7 @@ Section Dequeue.
     iIntros "!> (PH & DR & (%i & %r & %b & #ITHR & %BR & #TOKS))".
 
     wp_bind (Rec _ _ _)%E. do 3 pure_step_cases.
-    fold (get_to_free (SQ Head0 Tail0 BeingRead0 FreeLater0 OldHeadVal0)).
+    fold (get_to_free (SQ Head Tail BeingRead FreeLater OldHeadVal)).
     rewrite -Q_SQ. 
     wp_bind (get_to_free _ _)%E.         
     split_cps "CPS" (3 * get_loc_fuel); [cbv; lia| ].
